minor cleanup

examples/invariants/DY.Example.Invariants.Uniqueness.Injectivity.fst
@@ -1,5 +1,6 @@
 module DY.Example.Invariants.Uniqueness.Injectivity
 
+
 open DY.Example.Invariants.Uniqueness
 
 open Comparse
@@ -9,69 +10,6 @@ module Lib = DY.Lib
 module Trace = DY.Core.Trace.Type
 
 #set-options "--fuel 1 --ifuel 1"
-
-let rec sessions_history
-  (tr:trace) (p:principal) (sid:state_id):
-  Lemma
-  (requires has_session_for tr p sid
-  )
-  (ensures (
-    let Snoc init last = access_session tr p sid in
-
-    match init with
-    | Nil -> True
-    | _ -> 
-      let tr_before =(tr `prefix_before_event` (SetState p sid last)) in
-    has_session_for tr_before p sid
-    /\ init = access_session tr_before p sid
-  ))
-  (decreases (Trace.length tr))
-  = 
-  let Snoc init last = access_session tr p sid in
-  match init with
-  | Nil -> ()
-  | _ -> (
-    match tr with 
-    | Nil -> ()
-    | Snoc tr_init (SetState p' sid' cont') -> (
-        if p' = p && sid' = sid
-        then (
-      let tr_before =(tr `prefix_before_event` (SetState p sid last)) in
-      sessions_history tr_before p sid
-   )
-      else sessions_history tr_init p sid
-  )
-    | Snoc tr_init _ -> sessions_history tr_init p sid
-    )
-
-let rec session_mem_state_was_set
-  (tr:trace) (p:principal) (sid:state_id) (sess:session_raw) (cont:state_raw):
-  Lemma
-  (requires (
-     has_session_for tr p sid /\
-     sess = access_session tr p sid /\
-     cont `memP` sess
-  ))
-  (ensures (
-     let Snoc _ last = access_session tr p sid in
-
-     if cont = last
-     then True
-     else
-     state_was_set (tr `prefix_before_event` (SetState p sid last)) p sid cont
-  ))
-  (decreases Trace.length tr)
-  = 
-     let Snoc init last = access_session tr p sid in
-     if last = cont
-     then ()
-     else (
-     memP_singleton  last cont;
-     assert(Snoc? init);
-        sessions_history tr p sid;
-     session_mem_state_was_set (tr `prefix_before_event` (SetState p sid last)) p sid init cont
-     )
-
 #push-options "--z3rlimit 20"
 let rec session_has_same_idn1 
   (tr:trace) (p:principal) (sid:state_id) (cont:state_raw):
@@ -177,7 +115,6 @@ let state_injective_ (tr:trace)
    )
 #pop-options 
 
-#push-options "--z3rlimit 20 --fuel 4  --z3cliopt 'smt.qi.eager_threshold=20'"
 let state_injective (tr:trace)
   (p:principal)
   (sid sid': state_id)
